formalized metamath metatheory

Metamath/Translate.lean
@@ -3,8 +3,36 @@
 import Lean
 import Metamath.Verify
 
+open Or in
+theorem or_assoc {a b c} : (a ∨ b) ∨ c ↔ a ∨ (b ∨ c) :=
+⟨fun | inl (inl h) => inl h
+     | inl (inr h) => inr (inl h)
+     | inr h => inr (inr h),
+ fun | inl h => inl (inl h)
+     | inr (inl h) => inl (inr h)
+     | inr (inr h) => inr h⟩
+
+theorem Or.symm : a ∨ b → b ∨ a
+| Or.inl h => Or.inr h
+| Or.inr h => Or.inl h
+
+namespace List
+
+def mem (a : α) : List α → Prop
+| [] => False
+| (b :: l) => a = b ∨ mem a l
+
+infix:50 " ∈ " => mem
+
+theorem mem_append {a} : ∀ {l₁ l₂ : List α}, a ∈ l₁ ++ l₂ ↔ a ∈ l₁ ∨ a ∈ l₂
+| [], _ => by simp [mem]
+| b :: l₁, l₂ => by simp only [List.cons_append, mem, or_assoc, mem_append]; exact Iff.rfl
+
+end List
+
 namespace Metamath
 open Lean Elab
+open Verify in
 partial def foo : TermElabM Unit := do
   let mut s : ParserState := Inhabited.default
   s := s.withDB fun db => { db with interrupt := true }
@@ -30,73 +58,354 @@ partial def foo : TermElabM Unit := do
 
 -- #eval foo
 
-namespace Translate
+def CN := String
+instance : Inhabited CN := inferInstanceAs (Inhabited String)
+instance : DecidableEq CN := inferInstanceAs (DecidableEq String)
 
-def VR := Nat
-instance : BEq VR := inferInstanceAs (BEq Nat)
+structure VR := (type : CN) (i : Nat)
+deriving DecidableEq
 
 inductive Sym
-| const (c : String)
-| var (c : String) (n : VR)
-deriving Inhabited, BEq
+| const (c : CN)
+| var (n : VR)
+deriving Inhabited, DecidableEq
 open Sym
 
 instance : Coe String Sym := ⟨const⟩
 def Sym.isVar : Sym → Bool
 | const _ => false
-| var _ _ => true
+| var _ => true
 
-abbrev Formula := List Sym
+def Expr := List Sym
+def VR.expr (v : VR) : Expr := [var v]
 
-def Formula.δ (a b : Formula) : Bool :=
+instance : Append Expr := inferInstanceAs (Append (List Sym))
+def Expr.sn (s : Sym) : Expr := [s]
+instance : Coe String Expr := ⟨fun c => Expr.sn c⟩
+instance : Coe VR Expr := ⟨fun v => Expr.sn (var v)⟩
+def Expr.cons (c : String) : Expr → Expr := List.cons c
+def Expr.mem (e : Expr) (v : VR) : Prop := var v ∈ e
+
+scoped notation:50 a:51 " ∈' " b:51 => Expr.mem b a
+
+def Expr.subst (σ : VR → Expr) : Expr → Expr
+| [] => []
+| const c :: e => const c :: subst σ e
+| var v :: e => σ v ++ subst σ e
+
+theorem Expr.subst_id : (e : Expr) → Expr.subst VR.expr e = e
+| [] => rfl
+| const c :: e => congrArg (const c :: .) (subst_id e)
+| var v :: e => congrArg (var v :: .) (subst_id e)
+
+theorem Expr.subst_append (σ) : (e₁ e₂ : Expr) → Expr.subst σ (e₁ ++ e₂) = e₁.subst σ ++ e₂.subst σ
+| [], _ => rfl
+| const c :: (e₁ : Expr), e₂ => by
+  simp only [Expr.subst]; rw [List.cons_append, List.cons_append, ← subst_append]; rfl
+| var v :: e, e₂ => by
+  rw [List.cons_append]; simp only [Expr.subst]; rw [List.append_assoc, subst_append]
+
+theorem Expr.mem_subst {σ a} : {e : Expr} → a ∈' Expr.subst σ e → ∃ b, b ∈' e ∧ a ∈' σ b
+| const c :: (e : Expr), Or.inr h => let ⟨b, h₁, h₂⟩ := mem_subst h; ⟨b, Or.inr h₁, h₂⟩
+| var v :: e, h =>
+  match List.mem_append.1 h with
+  | Or.inl h => ⟨v, Or.inl rfl, h⟩
+  | Or.inr h => let ⟨b, h₁, h₂⟩ := mem_subst h; ⟨b, Or.inr h₁, h₂⟩
+
+def subst.trans (σ σ' : VR → Expr) (v : VR) : Expr := (σ v).subst σ'
+
+theorem Expr.subst_tr (σ σ' : VR → Expr) : (e : Expr) →
+  e.subst (subst.trans σ σ') = (e.subst σ).subst σ'
+| [] => rfl
+| const c :: e => congrArg (const c :: .) (subst_tr _ _ e)
+| var v :: e => by simp only [subst]; rw [subst_append, subst_tr]; rfl
+
+def Formula := CN × Expr
+
+def Formula.subst (σ : VR → Expr) : Formula → Formula
+| (c, e) => (c, e.subst σ)
+
+theorem Formula.subst_id : (e : Formula) → Formula.subst VR.expr e = e
+| (c, e) => congrArg (c, .) e.subst_id
+
+theorem Formula.subst_tr (σ σ' : VR → Expr) : (e : Formula) →
+  e.subst (subst.trans σ σ') = (e.subst σ).subst σ'
+| (c, e) => congrArg (c, .) (e.subst_tr _ _)
+
+def VR.vhyp (v : VR) : Formula := (v.type, [var v])
+instance : Coe VR Formula := ⟨VR.vhyp⟩
+
+def Expr.δ (a b : Expr) : Bool :=
 a.all fun
 | const _ => true
-| var _ a => b.all fun
+| var a => b.all fun
   | const _ => true
-  | var _ b => a != b
+  | var b => a != b
 
-def ze : Formula := ["0"]
-def pl (t r : Formula) := ↑"(" :: t ++ ↑"+" :: r ++ [↑")"]
-def eq (t r : Formula) := t ++ ↑"=" :: r
-def im (P Q : Formula) := ↑"(" :: P ++ ↑"->" :: Q ++ [↑")"]
-def al (x P : Formula) := ↑"A." :: x ++ P
+structure DJ :=
+  disj : VR → VR → Prop
+  irr : ¬ disj x x
+  symm : disj x y → disj y x
 
-class Proof where
-  ρ : Sym → Formula → Prop
-open Proof
+instance : CoeFun DJ (fun _ => VR → VR → Prop) := ⟨DJ.disj⟩
 
+def DJ.mk' (disj : List (VR × VR)) : DJ :=
+{ disj := fun a b => a ≠ b ∧ ((a, b) ∈ disj ∨ (b, a) ∈ disj)
+  irr := fun h => h.1 rfl
+  symm := fun ⟨h, h'⟩ => ⟨h.symm, h'.symm⟩ }
+
+def Expr.disjoint (dj : DJ) (e₁ e₂ : Expr) : Prop :=
+  ∀ c d, c ∈' e₁ → d ∈' e₂ → dj c d
+
+def DJ.subst (σ : VR → Expr) (dj dj' : DJ) :=
+  ∀ a b, dj a b → (σ a).disjoint dj' (σ b)
+
+structure Context :=
+  hyps : Formula → Prop
+  dj : DJ
+
+def Context.mk' (disj : List (VR × VR)) (hyps : List Formula) : Context :=
+  ⟨fun h => h ∈ hyps, DJ.mk' disj⟩
+
+structure Statement :=
+  ctx : Context
+  fmla : Formula
+
+inductive Provable (axioms : Statement → Prop) (Γ : Context) : Formula → Prop
+| hyp (h) : Γ.hyps h → Provable axioms Γ h
+| var (v:VR) : Provable axioms Γ v
+| ax (σ : VR → Expr) {ax} : axioms ax → ax.ctx.dj.subst σ Γ.dj →
+  (∀ h, ax.ctx.hyps h ∨ (∃ v:VR, h = v) → Provable axioms Γ (h.subst σ)) →
+  Provable axioms Γ (ax.fmla.subst σ)
+
+def Statement.provable (axioms : Statement → Prop) (s : Statement) : Prop :=
+  Provable axioms s.ctx s.fmla
+
+theorem Provable.ax_self (axioms : Statement → Prop)
+  {ax} (H : axioms ax) : ax.provable axioms := by
+  have _ from Provable.ax (Γ := ax.ctx) VR.expr H ?disj ?hyp
+  rw [Formula.subst_id] at this; exact this
+  case disj =>
+    intro a b h a' b' h₁ h₂
+    match a', b', h₁, h₂ with | _, _, Or.inl rfl, Or.inl rfl => ?_
+    exact h
+  case hyp =>
+    intro fmla h
+    match fmla, h with
+    | fmla, Or.inl h => rw [Formula.subst_id]; exact Provable.hyp _ h
+    | _, Or.inr ⟨v, rfl⟩ => exact Provable.var v
+
+theorem Provable.trans' {axioms : Statement → Prop} {Γ : Context}
+  (σ : VR → Expr) {Γ' fmla} (pr : Provable axioms Γ' fmla)
+  (dj : Γ'.dj.subst σ Γ.dj)
+  (hh : ∀ h, Γ'.hyps h ∨ (∃ v:VR, h = v) → Provable axioms Γ (h.subst σ)) :
+  Provable axioms Γ (fmla.subst σ) := by
+  induction pr with
+  | hyp f h => exact hh _ (Or.inl h)
+  | var v => exact hh _ (Or.inr ⟨v, rfl⟩)
+  | @ax σ' a ha dj' hh' IH =>
+    rw [← Formula.subst_tr]
+    apply ax (subst.trans σ' σ) ha
+    focus
+      intros a b ab c d hc hd
+      let ⟨e, ea, ce⟩ := Expr.mem_subst hc
+      let ⟨f, fb, df⟩ := Expr.mem_subst hd
+      refine dj _ _ ?_ _ _ ce df
+      exact dj' _ _ ab _ _ ea fb
+    focus { intros f; rw [Formula.subst_tr]; refine IH _ }
+
+theorem Provable.trans {axioms : Statement → Prop} {Γ : Context}
+  (σ : VR → Expr) (s : Statement) : s.provable axioms →
+  s.ctx.dj.subst σ Γ.dj →
+  (∀ h, s.ctx.hyps h ∨ (∃ v:VR, h = v) → Provable axioms Γ (h.subst σ)) →
+  Provable axioms Γ (s.fmla.subst σ) :=
+  Provable.trans' (axioms := axioms) σ
+
+def subst_of : List (VR × Expr) → VR → Expr
+| [], v => v
+| (a, e)::l, v => if a = v then e else subst_of l v
+
+class Subst (σ : VR → Expr) (e : Expr) (e' : outParam Expr) := (out : e.subst σ = e')
+
+instance [Subst σ e₁ e₁'] [Subst σ e₂ e₂'] : Subst σ (e₁ ++ e₂) (e₁' ++ e₂') :=
+  ⟨by rw [Expr.subst_append, Subst.out, Subst.out]⟩
+
+instance (s : String) : Subst σ s s := ⟨rfl⟩
+
+instance (s : String) [Subst σ e e'] : Subst σ (s ++ e) (s ++ e') :=
+  inferInstanceAs (Subst σ (Expr.sn _ ++ e) _)
+instance (s : String) [Subst σ e e'] : Subst σ (e ++ s) (e' ++ s) :=
+  inferInstanceAs (Subst σ (e ++ Expr.sn _) _)
+
+def subst.ok (axs Γ) (σ : VR → Expr) := ∀ v, Provable axs Γ (v.type, σ v)
+
+theorem subst.ok.nil {axs Γ} : subst.ok axs Γ (subst_of []) := Provable.var
+theorem subst.ok.cons {axs Γ e σ} (x) (h₁ : Provable axs Γ (x.type, e))
+  (h₂ : subst.ok axs Γ (subst_of σ)) : subst.ok axs Γ (subst_of ((x, e)::σ)) := by
+  intro v
+  simp only [subst_of]
+  cases Decidable.em (x = v) with simp [h]
+  | inl h => cases h; exact h₁
+  | inr h => exact h₂ v
+
+theorem Provable.thm {axs} {Γ : Context}
+  {σ : VR → Expr} {dj hyps c s} (pr : Provable axs (Context.mk' dj hyps) (c, s))
+  (hv : subst.ok axs Γ σ)
+  (dj : (DJ.mk' dj).subst σ Γ.dj)
+  (hh : ∀ h, h ∈ hyps → Provable axs Γ (h.subst σ))
+  {e} [inst : Subst σ s e] : Provable axs Γ (c, e) := by
+  rw [← inst.out]
+  exact Metamath.Provable.trans' σ pr dj fun
+    | f, Or.inl h => hh _ h
+    | _, Or.inr ⟨v, rfl⟩ =>
+      show Provable axs Γ (v.type, σ v ++ show Expr from []) by
+      rw [List.append_nil]; exact hv v
+
+theorem DJ_nil {σ dj'} : (DJ.mk' []).subst σ dj' | _, _, h => nomatch h
+theorem DJ_cons {a b l σ dj'}
+  (h₁ : (σ a).disjoint dj' (σ b))
+  (h₂ : (DJ.mk' l).subst σ dj') : (DJ.mk' ((a, b) :: l)).subst σ dj'
+| _, _, ⟨_, Or.inl (Or.inl rfl)⟩ => h₁
+| _, _, ⟨_, Or.inr (Or.inl rfl)⟩ => fun x y hx hy => dj'.symm (h₁ y x hy hx)
+| _, _, ⟨h, Or.inl (Or.inr h')⟩ => h₂ _ _ ⟨h, Or.inl h'⟩
+| _, _, ⟨h, Or.inr (Or.inr h')⟩ => h₂ _ _ ⟨h, Or.inr h'⟩
+
+theorem HH_nil {axs Γ σ} : ∀ h:Formula, h ∈ [] → Provable axs Γ (h.subst σ)
+| _, h => nomatch h
+
+theorem HH_cons {axs Γ σ c f hyps}
+  {e} [Subst σ f e] (h₁ : Provable axs Γ (c, e))
+  (h₂ : ∀ h:Formula, h ∈ hyps → Provable axs Γ (h.subst σ)) :
+  ∀ h:Formula, h ∈ (c, f)::hyps → Provable axs Γ (h.subst σ)
+| _, Or.inl rfl => by rw [← @Subst.out σ f e] at h₁; exact h₁
+| _, Or.inr h => h₂ _ h
+
+class Typed (axs : outParam _) (c : outParam CN) (e : Expr) :=
+  type (Γ) : Provable axs Γ (c, e)
+
+def Expr.ty (e) {axs c} [Typed axs c e] {Γ} : Provable axs Γ (c, e) := Typed.type Γ
 -- This is a by hand translation of demo0.mm, ideally the tactic will write this
 
-def Set [Proof] := {t // ρ "set" t}
-def Term [Proof] := {t // ρ "term" t}
-def Wff [Proof] := {t // ρ "wff" t}
+namespace Demo
 
-def Prf [Proof] (P : Wff) : Prop := ρ "|-" P.1
-prefix "⊢" => Prf
+def ze : Expr := "0"
+instance : Subst σ ze ze := inferInstanceAs (Subst σ "0" _)
 
-class Database extends Proof where
-  tze : ρ "term" ze
-  tpl : ∀ {t r}, ρ "term" t → ρ "term" r → ρ "term" (pl t r)
-  weq : ∀ {t r}, ρ "term" t → ρ "term" r → ρ "wff" (eq t r)
-  wim : ∀ {P Q}, ρ "wff" P → ρ "wff" Q → ρ "wff" (im P Q)
-  wal : ∀ {x P}, ρ "set" x → ρ "wff" P → ρ "wff" (al x P)
-  a1 : ∀ {t r s}, ρ "term" t → ρ "term" r → ρ "term" s → ρ "|-" (im (eq t r) (im (eq t s) (eq r s)))
-  a2 : ∀ {t}, ρ "term" t → ρ "|-" (eq (pl t ze) t)
-  mp : ∀ {P Q}, ρ "wff" P → ρ "wff" Q → ρ "|-" P → ρ "|-" (im P Q) → ρ "|-" Q
-  ax5 : ∀ {x P}, ρ "set" x → ρ "wff" P → x.δ P → ρ "|-" (im P (al x P))
+def pl (t r : Expr) : Expr := "(" ++ t ++ "+" ++ r ++ ")"
+instance [Subst σ t t'] [Subst σ r r'] : Subst σ (pl t r) (pl t' r') :=
+  inferInstanceAs (Subst σ (_++_) _)
 
-namespace Database
-variable [Database]
+def eq (t r : Expr) : Expr := t ++ "=" ++ r
+instance [Subst σ t t'] [Subst σ r r'] : Subst σ (eq t r) (eq t' r') :=
+  inferInstanceAs (Subst σ (_++_) _)
 
-def Ze : Term := ⟨ze, tze⟩
-def Pl (t r : Term) : Term := ⟨_, tpl t.2 r.2⟩
-def Eq (t r : Term) : Wff := ⟨_, weq t.2 r.2⟩
-def Im (P Q : Wff) : Wff := ⟨_, wim P.2 Q.2⟩
-def Al (x : Set) (P : Wff) : Wff := ⟨_, wal x.2 P.2⟩
-def A1 {t r s} : ⊢ Im (Eq t r) (Im (Eq t s) (Eq r s)) := a1 t.2 r.2 s.2
-def A2 {t} : ⊢ Eq (Pl t Ze) t := a2 t.2
-def Mp {P Q} (h1 : ⊢ P) (h2 : ⊢ Im P Q) : ⊢ Q := mp P.2 Q.2 h1 h2
+def im (P Q : Expr) : Expr := "(" ++ P ++ "->" ++ Q ++ ")"
+instance {P Q P' Q'} [Subst σ P P'] [Subst σ Q Q'] : Subst σ (im P Q) (im P' Q') :=
+  inferInstanceAs (Subst σ (_++_) _)
 
-theorem th1 {t} : ⊢ Eq t t := Mp A2 (Mp A2 A1)
+def al (x P : Expr) : Expr := "A." ++ x ++ P
+instance {x P x' P'} [Subst σ x x'] [Subst σ P P'] : Subst σ (al x P) (al x' P') :=
+  inferInstanceAs (Subst σ (_++_) _)
 
-end Database
+def vt : VR := ⟨"term", 0⟩
+def vr : VR := ⟨"term", 1⟩
+def vs : VR := ⟨"term", 2⟩
+def vP : VR := ⟨"wff", 0⟩
+def vQ : VR := ⟨"wff", 1⟩
+def vx : VR := ⟨"set", 0⟩
+
+def axioms (s : Statement) : Prop := s ∈ [
+  ⟨Context.mk' [] [], ("term", ze)⟩,
+  ⟨Context.mk' [] [], ("term", pl vt vr)⟩,
+  ⟨Context.mk' [] [], ("wff", eq vt vr)⟩,
+  ⟨Context.mk' [] [], ("wff", im vP vQ)⟩,
+  ⟨Context.mk' [] [], ("wff", al vx vP)⟩,
+  ⟨Context.mk' [] [], ("|-", im (eq vt vr) (im (eq vt vs) (eq vr vs)))⟩,
+  ⟨Context.mk' [] [], ("|-", eq (pl vt ze) vt)⟩,
+  ⟨Context.mk' [] [("|-", vP), ("|-", im vP vQ)], ("|-", vQ)⟩,
+  ⟨Context.mk' [(vx, vP)] [], ("|-", im vP (al vx vP))⟩
+]
+
+abbrev Provable := Metamath.Provable axioms
+abbrev Typed := Metamath.Typed axioms
+
+instance tze : Typed "term" ze :=
+⟨fun Γ =>
+  (Provable.ax_self axioms (Or.inl rfl)).thm subst.ok.nil DJ_nil HH_nil⟩
+
+instance tpl {t r} [Typed "term" t] [Typed "term" r] :
+  Typed "term" (pl t r) :=
+⟨fun Γ =>
+  have Subst (subst_of [(vt, t), (vr, r)]) vt t from ⟨List.append_nil _⟩
+  have Subst (subst_of [(vt, t), (vr, r)]) vr r from ⟨List.append_nil _⟩
+  (Provable.ax_self axioms (Or.inr $ Or.inl rfl)).thm
+    (subst.ok.cons vt t.ty $ subst.ok.cons vr r.ty subst.ok.nil)
+    DJ_nil HH_nil⟩
+
+instance weq {t r} [Typed "term" t] [Typed "term" r] :
+  Typed "wff" (eq t r) :=
+⟨fun Γ =>
+  have Subst (subst_of [(vt, t), (vr, r)]) vt t from ⟨List.append_nil _⟩
+  have Subst (subst_of [(vt, t), (vr, r)]) vr r from ⟨List.append_nil _⟩
+  (Provable.ax_self axioms (Or.inr $ Or.inr $ Or.inl rfl)).thm
+    (subst.ok.cons vt t.ty $ subst.ok.cons vr r.ty subst.ok.nil)
+    DJ_nil HH_nil⟩
+
+instance wim {P Q} [Typed "wff" P] [Typed "wff" Q] :
+  Typed "wff" (im P Q) :=
+⟨fun Γ =>
+  have Subst (subst_of [(vP, P), (vQ, Q)]) vP P from ⟨List.append_nil _⟩
+  have Subst (subst_of [(vP, P), (vQ, Q)]) vQ Q from ⟨List.append_nil _⟩
+  (Provable.ax_self axioms (Or.inr $ Or.inr $ Or.inr $ Or.inl rfl)).thm
+    (subst.ok.cons vP P.ty $ subst.ok.cons vQ Q.ty subst.ok.nil)
+    DJ_nil HH_nil⟩
+
+instance wal {x P} [Typed "set" x] [Typed "wff" P] :
+  Typed "wff" (al x P) :=
+⟨fun Γ =>
+  have Subst (subst_of [(vx, x), (vP, P)]) vx x from ⟨List.append_nil _⟩
+  have Subst (subst_of [(vx, x), (vP, P)]) vP P from ⟨List.append_nil _⟩
+  (Provable.ax_self axioms (Or.inr $ Or.inr $ Or.inr $ Or.inr $ Or.inl rfl)).thm
+    (subst.ok.cons vx x.ty $ subst.ok.cons vP P.ty subst.ok.nil)
+    DJ_nil HH_nil⟩
+
+theorem a1 {Γ t r s} [Typed "term" t] [Typed "term" r] [Typed "term" s] :
+  Provable Γ ("|-", im (eq t r) (im (eq t s) (eq r s))) :=
+  have Subst (subst_of [(vt, t), (vr, r), (vs, s)]) vt t from ⟨List.append_nil _⟩
+  have Subst (subst_of [(vt, t), (vr, r), (vs, s)]) vr r from ⟨List.append_nil _⟩
+  have Subst (subst_of [(vt, t), (vr, r), (vs, s)]) vs s from ⟨List.append_nil _⟩
+  (Provable.ax_self axioms (Or.inr $ Or.inr $ Or.inr $ Or.inr $ Or.inr $ Or.inl rfl)).thm
+    (subst.ok.cons vt t.ty $ subst.ok.cons vr r.ty $ subst.ok.cons vs s.ty subst.ok.nil)
+    DJ_nil HH_nil
+
+theorem a2 {Γ t} [Typed "term" t] :
+  Provable Γ ("|-", eq (pl t ze) t) :=
+  have Subst (subst_of [(vt, t)]) vt t from ⟨List.append_nil _⟩
+  (Provable.ax_self axioms (Or.inr $ Or.inr $ Or.inr $ Or.inr $ Or.inr $ Or.inr $ Or.inl rfl)).thm
+    (subst.ok.cons vt t.ty subst.ok.nil)
+    DJ_nil HH_nil
+
+theorem mp {Γ P Q} [Typed "wff" P] [Typed "wff" Q]
+  (min : Provable Γ ("|-", P))
+  (maj : Provable Γ ("|-", im P Q)) :
+  Provable Γ ("|-", Q) :=
+  have Subst (subst_of [(vP, P), (vQ, Q)]) vP P from ⟨List.append_nil _⟩
+  have Subst (subst_of [(vP, P), (vQ, Q)]) vQ Q from ⟨List.append_nil _⟩
+  (Provable.ax_self axioms (Or.inr $ Or.inr $ Or.inr $ Or.inr $ Or.inr $ Or.inr $ Or.inr $ Or.inl rfl)).thm
+    (subst.ok.cons vP P.ty $ subst.ok.cons vQ Q.ty subst.ok.nil)
+    DJ_nil (HH_cons min $ HH_cons maj HH_nil)
+
+theorem ax5 {Γ x P} [Typed "set" x] [Typed "wff" P]
+  (xp : x.disjoint Γ.dj P) :
+  Provable Γ ("|-", im P (al x P)) :=
+  have Subst (subst_of [(vx, x), (vP, P)]) vx x from ⟨List.append_nil _⟩
+  have Subst (subst_of [(vx, x), (vP, P)]) vP P from ⟨List.append_nil _⟩
+  (Provable.ax_self axioms (Or.inr $ Or.inr $ Or.inr $ Or.inr $ Or.inr $ Or.inr $ Or.inr $ Or.inr $ Or.inl rfl)).thm
+    (subst.ok.cons vx x.ty $ subst.ok.cons vP P.ty subst.ok.nil)
+    (DJ_cons xp DJ_nil) HH_nil
+
+theorem th1 {Γ t} [Typed "term" t] :
+  Provable Γ ("|-", eq t t) := mp a2 (mp a2 a1)
+
+end Demo
+end Metamath
