Metamath.lean
@@ -1,6 +1,6 @@
 import Metamath.Verify
 
-open Metamath in
+open Metamath.Verify in
 def main (n : List String) : IO UInt32 := do
   let db ← check $ n.getD 0 "set.mm"
   match db.error? with
